#228 step-lemma for medUnfair, final proof with oops

abp/Medium/medUnfairAut.thy
@@ -1,27 +1,28 @@
 theory medUnfairAut
 
-imports PreludeMed automat.ndAutomaton
+imports PreludeMed automat.ndAutomaton automat.ndaTotal
 
 begin
 
 
+datatype medState = Single
+
 (* Superset of the Fair-Transition *)
 fun medUnfairTransitionH :: "medState \<Rightarrow> 'a tsyn \<Rightarrow> (medState \<times> 'a tsyn) set" where
-"medUnfairTransitionH  state     -    = { (state,    -   )            }" |
-"medUnfairTransitionH (Suc n) (Msg m) = { (  n  ,    -   )            }" |
-"medUnfairTransitionH    0    (Msg m) = { (  n  , (Msg m)) | n . True } \<union> { (0, -) }"
+"medUnfairTransitionH  _      -    = { (Single,    -   )            }" |
+"medUnfairTransitionH  _   (Msg m) = { (Single  ,    -   ),  (Single  ,    Msg m  ) }"
 
 fun medUnfairTransition :: "(medState \<times> 'a mediumMessage tsyn sbElem) \<Rightarrow> ((medState \<times> 'a mediumMessage tsyn SB) set rev)" where
 "medUnfairTransition (s,f) = (if sbeDom f = mediumDom then 
     Rev ((\<lambda>(s,out). (s, mediumOut_o out)) ` (medUnfairTransitionH s (mediumElem_get_i f))) 
-  else undefined)"
+  else Rev { undefined })"
 
 lift_definition medUnfairAut :: "(medState, 'a mediumMessage tsyn) ndAutomaton" is 
-  "(medUnfairTransition, Rev {(n, mediumOut_o - )| n. True}, Discr mediumDom, Discr mediumRan)"
+  "(medUnfairTransition, Rev {(Single, mediumOut_o - )}, Discr mediumDom, Discr mediumRan)"
   by (simp add: mediumDom_def)
 
-definition medUnfair :: "medState \<Rightarrow> 'a mediumMessage tsyn SPS" where
-"medUnfair n = nda_h medUnfairAut n"
+definition medUnfair :: "'a mediumMessage tsyn SPS" where
+"medUnfair = nda_h medUnfairAut Single"
 
 
 
@@ -34,14 +35,57 @@ lemma medunfairaut_ran[simp]: "ndaRan\<cdot>medUnfairAut = mediumRan"
   by (simp add: medUnfairAut.rep_eq ndaRan.rep_eq)
 
 
-lemma medunfair_transition_tick [simp]: "medUnfairTransition (state, (mediumElemIn_i -)) = Rev {(state, mediumOut_o -)}"
+lemma medunfair_transition_tick [simp]: "medUnfairTransition (state, (mediumElemIn_i -)) = Rev {(Single, mediumOut_o -)}"
   by simp
 
-lemma medunfair_transition_msg_suc [simp]: "medUnfairTransition (Suc n, (mediumElemIn_i (Msg m))) = Rev {(n, mediumOut_o -)}"
+lemma medunfair_transition_msg [simp]: "medUnfairTransition (state, (mediumElemIn_i (Msg m))) = Rev {(Single, mediumOut_o -), (Single, mediumOut_o (Msg m))}"
   by simp
 
-lemma medunfair_transition_msg_0 [simp]: "medUnfairTransition (0, (mediumElemIn_i (Msg m))) = Rev ({(n, mediumOut_o (Msg m)) | n. True} \<union> { (0, mediumOut_o -) })"
-  by auto
 
+lemma medunfair_trans_total_h: "medUnfairTransition (Single, s) \<noteq> Rev {}"
+  apply(cases "sbeDom s = mediumDom", simp_all)
+  by (metis insert_not_empty medUnfairTransitionH.elims)
+
+lemma medunfair_trans_total[simp]: "(ndaTransition\<cdot>medUnfairAut) s \<noteq> Rev {}"
+  apply(simp add: ndaTransition_def medUnfairAut.rep_eq)
+  by (metis medState.exhaust medUnfairTransition.cases medunfair_trans_total_h)
+
+lemma medunfair_initial_total [simp]: "ndaInitialState\<cdot>medUnfairAut \<noteq> Rev {}"
+  by(simp add: ndaInitialState_def medUnfairAut.rep_eq)
+
+lemma medunfair_consistent[simp]: "uspecIsConsistent (nda_h medUnfairAut s)"
+  apply(rule nda_consistent)
+  by simp_all
+
+lemma medunfair_step_tick [simp]: "spsConcIn (mediumIn_i -) medUnfair = spsConcOut(mediumOut_o -) medUnfair"
+  apply(simp add: mediumIn_i_def medUnfair_def)
+  apply(rule nda_h_one_I, simp_all)
+   apply (simp add: medUnfairAut.rep_eq ndaTransition.rep_eq)
+  by (auto simp add: one_lnat_def)
+
+lemma medunfair_step_msg [simp]: "spsConcIn (mediumIn_i (Msg m)) medUnfair 
+  = ndaConcOutFlatten mediumDom mediumRan (Rev {(Single, mediumOut_o -), (Single, mediumOut_o (Msg m))}) (\<lambda>s. medUnfair)"
+  apply(simp add: medUnfair_def mediumIn_i_def)
+  apply(subst nda_h_I, auto)
+  apply(simp add: ndaTransition_def medUnfairAut.rep_eq)
+  by (metis medState.exhaust)
+
+
+lemma sps2spf_step_single: assumes "spsConcIn input sps = spsConcOut output sps2"
+          and "spf \<in> uspecSet sps"
+        obtains spf2 where "spfConcIn input\<cdot>spf = spfConcOut output\<cdot>spf2" and "spf2 \<in> uspecSet sps2"
+  oops
+
+lemma medunfair_spf_step_tick [simp]: assumes "spf \<in> uspecSet (medUnfair)"
+  shows "spfConcIn (mediumIn_i -)\<cdot>spf = spfConcOut (mediumOut_o -)\<cdot>spf"
+  oops
+
+(* Final Proof *)
+lemma medunfair_dom [simp]: assumes "spf \<in> uspecSet medUnfair"
+  shows "tsynDom\<cdot>(medium_get_stream_o\<cdot>(spf \<rightleftharpoons> mediumIn_stream_i\<cdot>s)) \<subseteq> tsynDom\<cdot>s"
+  using assms apply(induction s arbitrary: spf rule:ind)
+  apply(rule admI)
+    apply auto
+  oops
 
 end
